TransVal/terminates.v
@@ -3,11 +3,20 @@ Require Import IL.
 Set Implicit Arguments.
 
 Inductive terminates :onv val ->stmt -> onv val -> stmt -> Prop :=
-|terminatesReturn E e : terminates E (stmtReturn e) E (stmtReturn e)
-|terminatesCall E f e : terminates E (stmtGoto f e) E (stmtGoto f e)
-|terminatesCondT E c t f E' s : terminates E t E' s -> val2bool (match exp_eval E c with| Some v => v | _ => val_false end ) = true -> terminates E (stmtIf c t f) E' s
-|terminatesCondF E c t f E' s: terminates E f E' s -> val2bool (match exp_eval E c with |Some v => v |_ => val_false end)  = false -> terminates E (stmtIf c t f) E' s
-|terminatesLet E x e s E' s': terminates E s E' s' -> terminates E (stmtExp x e s) E' s'.
+|terminatesReturn E e 
+ : terminates E (stmtReturn e) E (stmtReturn e)
+|terminatesCall E f e 
+ : terminates E (stmtGoto f e) E (stmtGoto f e)
+|terminatesCondT E c v t f E' s 
+ : terminates E t E' s 
+-> exp_eval E c = Some v 
+-> val2bool v = true -> terminates E (stmtIf c t f) E' s
+|terminatesCondF E c v t f E' s
+: terminates E f E' s 
+  -> exp_eval E c = Some v
+  -> val2bool v = false -> terminates E (stmtIf c t f) E' s
+|terminatesLet E x e v s E' s'
+ : exp_eval E e = v -> terminates (E[x<- v]) s E' s' -> terminates E (stmtExp x e s) E' s'.
 
 (*
 *** Local Variables: ***
